\textbf{Lemma} \\[5pt]
For any boolean values \( a \) and \( b \):
\[
\neg (a \lor b) \Leftrightarrow (\neg a \land \neg b)
\]

\textbf{Proof.} \\[5pt]
We need to show both directions of the equivalence:
\[
\neg (a \lor b) \Rightarrow (\neg a \land \neg b) \quad \text{and} \quad (\neg a \land \neg b) \Rightarrow \neg (a \lor b)
\]

\textbf{First Direction:} \( \neg (a \lor b) \Rightarrow (\neg a \land \neg b) \)

1. Assume \( \neg (a \lor b) \).

2. To show \( \neg a \):
\begin{itemize}
	\item \textbf{Case} \( a = \text{true} \):
	\[
	a = \text{true} \Rightarrow a \lor b = \text{true} \Rightarrow \text{contradiction with } \neg (a \lor b).
	\]
	\item Therefore, \( \neg a \).
\end{itemize}

3. To show \( \neg b \):
\begin{itemize}
	\item \textbf{Case} \( b = \text{true} \):
	\[
	b = \text{true} \Rightarrow a \lor b = \text{true} \Rightarrow \text{contradiction with } \neg (a \lor b).
	\]
	\item Therefore, \( \neg b \).
\end{itemize}

4. We conclude that \( \neg (a \lor b) \Rightarrow (\neg a \land \neg b) \).

\textbf{Second Direction:} \( (\neg a \land \neg b) \Rightarrow \neg (a \lor b) \)

1. Assume \( \neg a \land \neg b \).

2. Consider \( a \lor b \):
\begin{itemize}
	\item \textbf{Case} \( a = \text{true} \): Contradicts \( \neg a \).
	\item \textbf{Case} \( b = \text{true} \): Contradicts \( \neg b \).
\end{itemize}

3. Therefore, \( (\neg a \land \neg b) \Rightarrow \neg (a \lor b) \).

\textbf{Conclusion:}
\[
\neg (a \lor b) \Leftrightarrow (\neg a \land \neg b)
\]

textbf{Lemma} \\[5pt]
For any boolean values \( a \) and \( b \):
\[
\neg (a \lor b) \Leftrightarrow (\neg a \land \neg b)
\]

\textbf{Proof.} \\[5pt]
\begin{align*}
	&\text{1. To prove:} \quad \neg (a \lor b) \Rightarrow (\neg a \land \neg b) \\
	&\quad \text{Assume:} \quad \neg (a \lor b) \\
	&\quad \text{Then, we have:} \\
	&\quad a = \text{true} \Rightarrow a \lor b = \text{true} \Rightarrow \bot \Rightarrow \neg a \\
	&\quad b = \text{true} \Rightarrow a \lor b = \text{true} \Rightarrow \bot \Rightarrow \neg b \\
	&\quad \therefore \neg a \land \neg b \\
	\\
	&\text{2. To prove:} \quad (\neg a \land \neg b) \Rightarrow \neg (a \lor b) \\
	&\quad \text{Assume:} \quad \neg a \land \neg b \\
	&\quad \text{Then,} \quad a \lor b = \text{true} \Rightarrow a = \text{true} \lor b = \text{true} \Rightarrow \bot \\
	&\quad \therefore \neg (a \lor b) \\
	\\
	&\text{Conclusion:} \quad \neg (a \lor b) \Leftrightarrow (\neg a \land \neg b)
\end{align*}
