\newpage
\subsection{Ambient Logic's Exercies: Level 2}

\begin{enumerate}[\textbf{[}\bfseries1\textbf{]}]
\item We want to prove that \( \neg (a \lor b) \implies \neg a \land \neg b \).
\[
\infer[\neg \text{Introduction}]{\neg a \land \neg b}{\neg (a \lor b)}
\]
\begin{proof}[\normalfont\text{[Part I]}]
\( \neg (a \lor b) \implies (\neg a \land \neg b) \)
\begin{enumerate}[Step 1.]
\item \( \neg (a \lor b) \) \hfill (Assumption)
\item Split the goal into two subgoals: \( \neg a \) and \( \neg b \).
\[
\infer[\to I]{\lnot(a\lor b)\;\to\;(\lnot a\;\land\;\lnot b)}
{
\infer[\land I]{\lnot a\;\land\;\lnot b}
{
\infer[\lnot I]{\lnot a}
{
\infer[\bot]{\bot}
{
\lnot(a\lor b)
&
\infer[\lor I]{a\lor b}{a}
}
}
&
\infer[\lnot I]{\lnot b}
{
\infer[\bot]{\bot}
{
\lnot(a\lor b)
&
\infer[\lor I]{a\lor b}{b}
}
}
}
}
\]

\end{enumerate}
\end{proof}
\begin{lstlisting}[style=easycrypt]
require import AllCore.  (* core theories *)
(* 
here's a lemma for learning some simple Ambient Logic proof techniques; 
in fact, it's already in EasyCrypt's library with the same name;  and smt() will prove it
*)

lemma negb_or (a b : bool) :
!(a \/ b) <=> !a /\ !b.
proof.
admit.
qed.
\end{lstlisting}
\begin{proof}[\sol]
\ \begin{center}
\begin{minipage}{.475\textwidth}
\[
\infer{\lnot(a \lor b) \;\to\; (\lnot a \;\land\; \lnot b)} {
\infer{\lnot a \;\land\; \lnot b} {
\infer{\lnot a} {
\infer{\bot} {
\lnot(a \lor b)
&
\infer{a \lor b}{a}
}
}
}
}
\]
\end{minipage}\hfill
\begin{minipage}{.475\textwidth}
\[
\infer{\lnot(a \lor b) \;\to\; (\lnot a \;\land\; \lnot b)}
{
\infer{\lnot a \;\land\; \lnot b}
{
\infer{\lnot a}
{
\infer{\bot}
{
\lnot(a \lor b)
&
\infer{a \lor b}{\text{\ecinline{case a.}}}
}
}
}
}
\]
\end{minipage}
\end{center}
\begin{center}
\begin{minipage}[t]{.275\textwidth}
\centering\ecinline{}
\begin{lstlisting}[style=normal]
Current goal

Type variables: <none>

a: bool
b: bool
-----------------------
! (a \/ b) <=> !a /\ !b
\end{lstlisting}
\vfill
\end{minipage}\hfill
\begin{minipage}[t]{.3\textwidth}
\centering\ecinline{split}
\begin{lstlisting}[style=normal]
Current goal (remaining: 2)

Type variables: <none>

a: bool
b: bool
----------------------
! (a \/ b) => !a /\ !b

Goal #2
----------------------
!a /\ !b => ! (a \/ b)
\end{lstlisting}
\end{minipage}\hfill
\begin{minipage}[t]{.3\textwidth}
\centering\ecinline{move => not_or}
\begin{lstlisting}[style=normal]
Current goal (remaining: 2)

Type variables: <none>

a: bool
b: bool
not_or: ! (a \/ b)
-----------------------
!a /\ !b

Goal #2
----------------------
!a /\ !b => ! (a \/ b)
\end{lstlisting}
\end{minipage}
\end{center}

\begin{center}
\begin{minipage}[t]{.3\textwidth}
\centering\ecinline{split}
\begin{lstlisting}[style=normal]
Current goal (remaining: 3)

Type variables: <none>

a: bool
b: bool
not_or: ! (a \/ b)
-----------------------
!a

Goal #2
----------------------
!b

Goal #3
----------------------
!a /\ !b => ! (a \/ b)
\end{lstlisting}
\vfill
\end{minipage}\hfill
\begin{minipage}[t]{.3\textwidth}
\centering\ecinline{case a}
\begin{lstlisting}[style=normal]
Current goal (remaining: 4)

Type variables: <none>

a: bool
b: bool
not_or: ! (a \/ b)
-----------------------
a => !true

Goal #2
----------------------
!a => !false

Goal #3
----------------------
!b

Goal #4
----------------------
!a /\ !b => ! (a \/ b)
\end{lstlisting}
\end{minipage}\hfill
\begin{minipage}[t]{.3\textwidth}
\centering\ecinline{move => a_true}
\begin{lstlisting}[style=normal]
Current goal (remaining: 4)

Type variables: <none>

a: bool
b: bool
not_or: ! (a \/ b)
a_true: a
-----------------------
!true

Goal #2
----------------------
!a => !false

Goal #3
----------------------
!b

Goal #4
----------------------
!a /\ !b => ! (a \/ b)
\end{lstlisting}
\end{minipage}
\end{center}


\ \color{gray!20}
\begin{lstlisting}[style=normal]
proof.
split.
(* proving ! (a \/ b) => !a /\ !b *)
move => not_or.
split.
case a.
move => a_true.
simplify.
have contrad : a \/ b.
left.
trivial.
trivial.
trivial.
case b.
move => b_true.
simplify.
have contrad : a \/ b.
right.
trivial.
trivial.
trivial.
(* proving !a /\ !b => ! (a \/ b) *)
move => and_not.
elim and_not => a_false b_false.
case (a \/ b).
move => or.
elim or.
trivial.
trivial.
trivial.
qed.
\end{lstlisting}
\end{proof}
\end{enumerate}

%\subsection*{Proof Part 1: \( \neg (a \lor b) \implies (\neg a \land \neg b) \)}
%
%
%
%\subsection*{Proof Part 2: \( (\neg a \land \neg b) \implies \neg (a \lor b) \)}
%
%\begin{proof}
%	\textbf{Goal}: Prove \( (\neg a \land \neg b) \implies \neg (a \lor b) \)
%	
%	\textbf{Step 1:} Assume \( \neg a \land \neg b \) \hfill (Assumption)
%	
%	\textbf{Step 2:} Eliminate the conjunction:
%	\[
%	\infer[\text{Conjunction Elimination}]{
%		\neg a \quad \text{and} \quad \neg b
%	}{
%		\neg a \land \neg b
%	}
%	\]
%	
%	\textbf{Step 3:} Assume \( a \lor b \) \hfill (Assumption for Negation)
%	
%	\textbf{Step 4:} Case analysis on \( a \lor b \):
%	
%	\[
%	\infer[\text{Case Analysis}]{
%		\bot
%	}{
%		\infer[\text{Assumption}]{
%			a
%		}{
%			a \lor b
%		},
%		\infer[\text{Negation Introduction}]{
%			\bot
%		}{
%			\neg a
%		}
%	}
%	\quad
%	\infer[\text{Case Analysis}]{
%		\bot
%	}{
%		\infer[\text{Assumption}]{
%			b
%		}{
%			a \lor b
%		},
%		\infer[\text{Negation Introduction}]{
%			\bot
%		}{
%			\neg b
%		}
%	}
%	\]
%	
%	\textbf{Step 5:} Since both cases lead to contradictions, conclude that \( \neg (a \lor b) \) follows by Negation Introduction.
%	
%\end{proof}
%
%\subsection*{Conclusion}
%Thus, we have proven the equivalence:
%\[
%\neg (a \lor b) \Leftrightarrow (\neg a \land \neg b)
%\]
%
%\[
%\infer[\text{Conjunction Introduction}]{
%	\neg a \land \neg b
%}{
%	\infer[\text{Negation Introduction}]{
%		\neg a
%	}{
%		\infer[\text{Assumption for Negation}]{
%			a \lor b
%		}{
%			\neg (a \lor b)
%		}
%	},
%	\infer[\text{Negation Introduction}]{
%		\neg b
%	}{
%		\infer[\text{Assumption for Negation}]{
%			a \lor b
%		}{
%			\neg (a \lor b)
%		}
%	}
%}\]